LeanDag.lean
@@ -2,3 +2,4 @@ import LeanDag.Validators
 import LeanDag.Block
 import LeanDag.BlockDag
 import LeanDag.CausalHistory
+import LeanDag.Persistence
